p256: wip: clean up Hacl.Impl.P256.Verify

code/ecdsap256/Hacl.Impl.P256.Verify.fst
@@ -10,23 +10,20 @@ open Lib.Buffer
 
 open Hacl.Spec.P256.Bignum
 open Hacl.Impl.P256.Bignum
-open Hacl.Impl.P256.Core
-open Hacl.Impl.P256.PointAdd
-open Hacl.Impl.P256.PointDouble
-open Hacl.Impl.P256.RawCmp
 open Hacl.Impl.P256.Point
 open Hacl.Impl.P256.Scalar
-open Hacl.Impl.P256.Qinv
 open Hacl.Impl.P256.PointMul
-open Hacl.Impl.P256.Constants
 
 open Hacl.Hash.SHA2
 open Spec.Hash.Definitions
 
+module LSeq = Lib.Sequence
+module BSeq = Lib.ByteSequence
+
 module S = Spec.P256
 module SM = Hacl.Spec.P256.MontgomeryMultiplication
-module BSeq = Lib.ByteSequence
 module PS = Hacl.Impl.P256.Sign
+module QI = Hacl.Impl.P256.Qinv
 
 #set-options "--z3rlimit 50 --fuel 0 --ifuel 0"
 
@@ -47,288 +44,100 @@ let are_r_and_s_valid r s =
 
 
 inline_for_extraction noextract
-val ecdsa_verification_step4:
-    bufferU1:lbuffer uint8 (size 32)
-  -> bufferU2: lbuffer uint8 (size 32)
-  -> r:felem
-  -> s:felem
-  -> hash:felem ->
-  Stack unit
-    (requires fun h ->
-      live h r /\ live h s /\ live h hash /\ live h bufferU1 /\ live h bufferU2 /\
-      disjoint bufferU1 bufferU2 /\
-      disjoint bufferU1 hash /\
-      disjoint bufferU1 r /\
-      disjoint bufferU1 s /\
-      disjoint bufferU2 hash /\
-      disjoint bufferU2 r /\
-      disjoint bufferU2 s /\
-      as_nat h s < S.order /\
-      as_nat h hash < S.order /\
-      as_nat h r < S.order
-    )
-    (ensures fun h0 _ h1 ->
-      modifies (loc bufferU1 |+| loc bufferU2) h0 h1 /\
-      (
-	let p0 = S.pow (as_nat h0 s) (S.order - 2) * as_nat h0 hash % S.order in
-	let p1 = S.pow (as_nat h0 s) (S.order - 2) * as_nat h0 r % S.order in
-	as_seq h1 bufferU1 == BSeq.nat_to_bytes_be 32 p0 /\
-	as_seq h1 bufferU2 == BSeq.nat_to_bytes_be 32 p1
-      )
-    )
+val ecdsa_verification_step4: u1:felem -> u2:felem -> r:felem -> s:felem -> z:felem -> Stack unit
+  (requires fun h ->
+    live h r /\ live h s /\ live h z /\ live h u1 /\ live h u2 /\
+    disjoint u1 u2 /\ disjoint u1 z /\ disjoint u1 r /\ disjoint u1 s /\
+    disjoint u2 z /\ disjoint u2 r /\ disjoint u2 s /\
+    as_nat h s < S.order /\ as_nat h z < S.order /\ as_nat h r < S.order)
+  (ensures fun h0 _ h1 -> modifies (loc u1 |+| loc u2) h0 h1 /\
+    as_nat h1 u1 == S.pow (as_nat h0 s) (S.order - 2) * as_nat h0 z % S.order /\
+    as_nat h1 u2 == S.pow (as_nat h0 s) (S.order - 2) * as_nat h0 r % S.order)
 
-let ecdsa_verification_step4 bufferU1 bufferU2 r s hash =
-  push_frame();
-  let h0 = ST.get() in
-    let tempBuffer = create (size 12) (u64 0) in
-    let inverseS = sub tempBuffer (size 0) (size 4) in
-    let u1 = sub tempBuffer (size 4) (size 4) in
-    let u2 = sub tempBuffer (size 8) (size 4) in
-
-    fromDomainImpl s inverseS;
-    qinv inverseS inverseS;
-    multPowerPartial s inverseS hash u1;
-    multPowerPartial s inverseS r u2;
-
-  let h1 = ST.get() in
-    bn_to_bytes_be4 u1 bufferU1;
-    bn_to_bytes_be4 u2 bufferU2;
-
-  let h2 = ST.get() in
-  pop_frame()
-
-
-
-inline_for_extraction noextract
-val ecdsa_verification_step5_0:
-    points:lbuffer uint64 (size 24)
-  -> pubKeyAsPoint: point
-  -> u1: lbuffer uint8 (size 32)
-  -> u2: lbuffer uint8 (size 32) ->
-  Stack unit
-    (requires fun h ->
-      live h points /\ live h pubKeyAsPoint /\ live h u1 /\ live h u2 /\
-      disjoint points u1 /\
-      disjoint points u2 /\
-      disjoint pubKeyAsPoint u1 /\
-      disjoint pubKeyAsPoint u2 /\
-      disjoint points pubKeyAsPoint /\
-      point_x_as_nat h pubKeyAsPoint < S.prime /\
-      point_y_as_nat h pubKeyAsPoint < S.prime /\
-      point_z_as_nat h pubKeyAsPoint < S.prime
-    )
-  (ensures fun h0 _ h1 ->
-    modifies (loc points) h0 h1 /\
-    as_nat h1 (gsub points (size 0) (size 4)) < S.prime /\
-    as_nat h1 (gsub points (size 4) (size 4)) < S.prime /\
-    as_nat h1 (gsub points (size 8) (size 4)) < S.prime /\
-    as_nat h1 (gsub points (size 12) (size 4)) < S.prime /\
-    as_nat h1 (gsub points (size 16) (size 4)) < S.prime /\
-    as_nat h1 (gsub points (size 20) (size 4)) < S.prime /\
-    (
-      let pointU1 = gsub points (size 0) (size 12) in
-      let pointU2 = gsub points (size 12) (size 12) in
-
-      let fromDomainPointU1 = SM.fromDomainPoint (as_point_nat h1 pointU1) in
-      let fromDomainPointU2 = SM.fromDomainPoint (as_point_nat h1 pointU2) in
-      let pointAtInfinity = (0, 0, 0) in
-      let u1D, _ = S.montgomery_ladder_spec (as_seq h0 u1) (pointAtInfinity, S.base_point) in
-      let u2D, _ = S.montgomery_ladder_spec (as_seq h0 u2) (pointAtInfinity, as_point_nat h0 pubKeyAsPoint) in
-      fromDomainPointU1 == u1D /\ fromDomainPointU2 == u2D
-    )
-  )
-
-let ecdsa_verification_step5_0 points pubKeyAsPoint u1 u2 =
+let ecdsa_verification_step4 u1 u2 r s z =
   push_frame ();
-  let u1_q = create_felem () in
-  let u2_q = create_felem () in
-  bn_from_bytes_be4 u1 u1_q;
-  bn_from_bytes_be4 u2 u2_q;
-  let pointU1G = sub points (size 0) (size 12) in
-  let pointU2Q = sub points (size 12) (size 12) in
-  point_mul_g pointU1G u1_q;
-  point_mul pointU2Q pubKeyAsPoint u2_q;
+  let inverseS = create_felem () in
+
+  fromDomainImpl s inverseS;
+  QI.qinv inverseS inverseS;
+  QI.multPowerPartial s inverseS z u1;
+  QI.multPowerPartial s inverseS r u2;
   pop_frame ()
 
 
 inline_for_extraction noextract
-val ecdsa_verification_step5_2:
-    pointSum: point
-  -> pubKeyAsPoint: point
-  -> u1: lbuffer uint8 (size 32)
-  -> u2: lbuffer uint8 (size 32) ->
-  Stack unit
-    (requires fun h ->
-      live h pointSum /\ live h pubKeyAsPoint /\ live h u1 /\ live h u2 /\
-      disjoint pointSum u1 /\
-      disjoint pointSum u2 /\
-      disjoint pubKeyAsPoint u1 /\
-      disjoint pubKeyAsPoint u2 /\
-      disjoint pubKeyAsPoint pointSum /\
-      point_x_as_nat h pubKeyAsPoint < S.prime /\
-      point_y_as_nat h pubKeyAsPoint < S.prime /\
-      point_z_as_nat h pubKeyAsPoint < S.prime
-    )
-    (ensures fun h0 _ h1 ->
-      modifies (loc pointSum |+| loc pubKeyAsPoint) h0 h1 /\
-      as_nat h1 (gsub pointSum (size 0) (size 4)) < S.prime /\
-      (
-        let pointAtInfinity = (0, 0, 0) in
-        let u1D, _ = S.montgomery_ladder_spec (as_seq h0 u1) (pointAtInfinity, S.base_point) in
-        let u2D, _ = S.montgomery_ladder_spec (as_seq h0 u2) (pointAtInfinity, as_point_nat h0 pubKeyAsPoint) in
-	let sumD =
-	  if  norm_jacob_point u1D = norm_jacob_point u2D
-	  then
-	    S.point_double u1D
-	  else
-	    S.point_add u1D u2D in
-        let pointNorm = S.norm_jacob_point sumD in
-        let resultPoint =  as_point_nat h1 pointSum in
-        pointNorm == resultPoint
-      )
-   )
+val ecdsa_verification_step5: x:felem -> pk:point -> u1:felem -> u2:felem -> Stack bool
+  (requires fun h ->
+    live h x /\ live h pk /\ live h u1 /\ live h u2 /\
+    disjoint x u1 /\ disjoint x u2 /\ disjoint x pk /\
+    disjoint pk u1 /\ disjoint pk u2 /\
+    point_inv h pk /\ as_nat h u1 < pow2 256 /\ as_nat h u2 < pow2 256)
+  (ensures fun h0 state h1 -> modifies (loc x |+| loc pk) h0 h1 /\
+    as_nat h1 x < S.prime /\
+   (let sumD = S.point_mul_double_g (as_nat h0 u1) (as_nat h0 u2) (as_point_nat h0 pk) in
+    let res = S.norm_jacob_point sumD in
+    let (res_x, _, _) = res in
+    state == not (S.is_point_at_inf res) /\
+    as_nat h1 x == res_x % S.order))
 
-
-let ecdsa_verification_step5_2 pointSum pubKeyAsPoint u1 u2 =
-  push_frame();
-  let points = create (size 24) (u64 0) in
-  let buff = create (size 88) (u64 0) in
-  ecdsa_verification_step5_0 points pubKeyAsPoint u1 u2;
-  let pointU1G = sub points (size 0) (size 12) in
-  let pointU2Q = sub points (size 12) (size 12) in
-
-  let equalX = is_point_eq_vartime pointU1G pointU2Q in
-  begin
-  if equalX then
-  	point_double pointU1G pointSum buff
-  else
-  	point_add pointU1G pointU2Q pointSum buff end;
+let ecdsa_verification_step5 x pk u1 u2 =
+  push_frame ();
+  let pointSum = create_point () in
+  point_mul_double_g pointSum u1 u2 pk;
   norm_jacob_point pointSum pointSum;
-  pop_frame()
-
-
-inline_for_extraction noextract
-val ecdsa_verification_step5:
-    x:felem
-  -> pubKeyAsPoint: point
-  -> u1: lbuffer uint8 (size 32)
-  -> u2: lbuffer uint8 (size 32) ->
-  Stack bool
-    (requires fun h ->
-      live h x /\ live h pubKeyAsPoint /\ live h u1 /\ live h u2 /\
-      disjoint x u1 /\
-      disjoint x u2 /\
-      disjoint pubKeyAsPoint u1 /\
-      disjoint pubKeyAsPoint u2 /\
-      disjoint x pubKeyAsPoint /\
-      point_x_as_nat h pubKeyAsPoint < S.prime /\
-      point_y_as_nat h pubKeyAsPoint < S.prime /\
-      point_z_as_nat h pubKeyAsPoint < S.prime
-    )
-    (ensures fun h0 state h1 ->
-      modifies (loc x |+| loc pubKeyAsPoint) h0 h1 /\
-      as_nat h1 x < S.prime /\
-      (
-        let pointAtInfinity = (0, 0, 0) in
-        let u1D, _ = S.montgomery_ladder_spec (as_seq h0 u1) (pointAtInfinity, S.base_point) in
-        let u2D, _ = S.montgomery_ladder_spec (as_seq h0 u2) (pointAtInfinity, as_point_nat h0 pubKeyAsPoint) in
-        let sumD =
-	  if  norm_jacob_point u1D = norm_jacob_point u2D
-	  then
-	    S.point_double u1D
-	  else
-	    S.point_add u1D u2D in
-        let pointNorm = S.norm_jacob_point sumD in
-        let (xResult, yResult, zResult) = pointNorm in
-        state == not (S.is_point_at_inf pointNorm) /\
-        as_nat h1 x == xResult % S.order
-    )
-  )
-
-let ecdsa_verification_step5 x pubKeyAsPoint u1 u2 =
-  push_frame();
-  let pointSum = create (size 12) (u64 0) in
-  ecdsa_verification_step5_2 pointSum pubKeyAsPoint u1 u2;
-  let resultIsPAI = is_point_at_inf_vartime pointSum in
-  let xCoordinateSum = sub pointSum (size 0) (size 4) in
-  copy x xCoordinateSum;
+  let is_res_point_at_inf = is_point_at_inf_vartime pointSum in
+  let res_x = getx pointSum in
+  copy x res_x;
   qmod_short x x;
-  pop_frame();
-  not resultIsPAI
+  pop_frame ();
+  not is_res_point_at_inf
 
 
 inline_for_extraction
 val ecdsa_verification_core:
-  alg:S.hash_alg_ecdsa
-  -> publicKeyPoint:point
-  -> hashAsFelem:felem
-  -> r:lbuffer uint64 (size 4)
-  -> s:lbuffer uint64 (size 4)
-  -> mLen:size_t{v mLen >= S.min_input_length alg}
-  -> m:lbuffer uint8 mLen
-  -> xBuffer:felem ->
+    alg:S.hash_alg_ecdsa
+  -> pk:point
+  -> z:felem
+  -> r:felem
+  -> s:felem
+  -> msg_len:size_t{v msg_len >= S.min_input_length alg}
+  -> msg:lbuffer uint8 msg_len
+  -> x:felem ->
   Stack bool
-    (requires fun h ->
-      live h publicKeyPoint /\ live h hashAsFelem /\ live h r /\ live h s /\ live h m /\ live h xBuffer /\
-      disjoint publicKeyPoint r /\
-      disjoint publicKeyPoint s /\
-      disjoint publicKeyPoint m /\
-      disjoint hashAsFelem r /\
-      disjoint hashAsFelem s /\
-      disjoint hashAsFelem m /\
-      disjoint xBuffer r /\
-      disjoint xBuffer s /\
-      disjoint xBuffer m /\
-      LowStar.Monotonic.Buffer.all_disjoint [loc publicKeyPoint; loc hashAsFelem; loc xBuffer] /\
-      as_nat h s < S.order /\ as_nat h r < S.order /\
-      point_x_as_nat h publicKeyPoint < S.prime /\
-      point_y_as_nat h publicKeyPoint < S.prime /\
-      point_z_as_nat h publicKeyPoint < S.prime
-    )
-    (ensures fun h0 state h1 ->
-      modifies (loc publicKeyPoint |+| loc hashAsFelem |+| loc xBuffer) h0 h1 /\
-       (
-	 let hashM = S.hash_ecdsa alg (v mLen) (as_seq h0 m) in
-	 let cutHashM = Lib.Sequence.sub hashM 0 32 in
-	 let hashNat =  BSeq.nat_from_bytes_be cutHashM % S.order in
+  (requires fun h ->
+    live h pk /\ live h z /\ live h r /\ live h s /\ live h msg /\ live h x /\
+    disjoint pk r /\ disjoint pk s /\ disjoint pk msg /\ disjoint z r /\
+    disjoint z s /\ disjoint z msg /\ disjoint x r /\ disjoint x s /\
+    disjoint x msg /\
+    LowStar.Monotonic.Buffer.all_disjoint [loc pk; loc z; loc x] /\
+    as_nat h s < S.order /\ as_nat h r < S.order /\
+    point_inv h pk)
+  (ensures fun h0 state h1 -> modifies (loc pk |+| loc z |+| loc x) h0 h1 /\
+    (let hashM = S.hash_ecdsa alg (v msg_len) (as_seq h0 msg) in
+    let z = BSeq.nat_from_bytes_be (LSeq.sub hashM 0 32) % S.order in
+    let u1 = S.pow (as_nat h0 s) (S.order - 2) * z % S.order in
+    let u2 = S.pow (as_nat h0 s) (S.order - 2) * as_nat h0 r % S.order in
+    let sumD = S.point_mul_double_g u1 u2 (as_point_nat h0 pk) in
+    let (res_x, _, _) = S.norm_jacob_point sumD in
+    state == not (S.is_point_at_inf (S.norm_jacob_point sumD)) /\
+    as_nat h1 x == res_x % S.order))
 
-         let p0 = S.pow (as_nat h0 s) (S.order - 2) * hashNat % S.order in
-	 let p1 = S.pow (as_nat h0 s) (S.order - 2) * as_nat h0 r % S.order in
-
-	 let bufferU1 = BSeq.nat_to_bytes_be 32 p0  in
-	 let bufferU2 = BSeq.nat_to_bytes_be 32 p1 in
-	 let pointAtInfinity = (0, 0, 0) in
-         let u1D, _ = S.montgomery_ladder_spec bufferU1 (pointAtInfinity, S.base_point) in
-         let u2D, _ = S.montgomery_ladder_spec bufferU2 (pointAtInfinity, as_point_nat h0 publicKeyPoint) in
-          let sumD =
-	  if  norm_jacob_point u1D = norm_jacob_point u2D
-	  then
-	    S.point_double u1D
-	  else
-	    S.point_add u1D u2D in
-         let (xResult, yResult, zResult) = S.norm_jacob_point sumD in
-         state == not (S.is_point_at_inf (S.norm_jacob_point sumD)) /\
-         as_nat h1 xBuffer == xResult % S.order
-      )
-  )
-
-let ecdsa_verification_core alg publicKeyBuffer hashAsFelem r s mLen m xBuffer =
-  push_frame();
-  let tempBufferU8 = create (size 64) (u8 0) in
-  let bufferU1 = sub tempBufferU8 (size 0) (size 32) in
-  let bufferU2 = sub tempBufferU8 (size 32) (size 32) in
-  PS.msg_as_felem alg mLen m hashAsFelem;
-  ecdsa_verification_step4  bufferU1 bufferU2 r s hashAsFelem;
-  let r = ecdsa_verification_step5 xBuffer publicKeyBuffer bufferU1 bufferU2 in
-  pop_frame();
+let ecdsa_verification_core alg pk z r s msg_len msg x =
+  push_frame ();
+  let u1 = create_felem () in
+  let u2 = create_felem () in
+  PS.msg_as_felem alg msg_len msg z;
+  ecdsa_verification_step4 u1 u2 r s z;
+  let r = ecdsa_verification_step5 x pk u1 u2 in
+  pop_frame ();
   r
 
 
 val ecdsa_verification_:
     alg:S.hash_alg_ecdsa
   -> public_key:lbuffer uint8 64ul
-  -> r_q:lbuffer uint64 4ul
-  -> s_q:lbuffer uint64 4ul
+  -> r_q:felem
+  -> s_q:felem
   -> msg_len:size_t{v msg_len >= S.min_input_length alg}
   -> msg:lbuffer uint8 msg_len ->
   Stack bool
@@ -339,8 +148,8 @@ val ecdsa_verification_:
 
 let ecdsa_verification_ alg public_key r_q s_q msg_len msg =
   push_frame ();
-  let hashAsFelem = create_felem () in
-  let xBuffer = create_felem () in
+  let z = create_felem () in
+  let x = create_felem () in
   let pk = create_point () in
 
   let publicKeyCorrect = load_point_vartime pk public_key in
@@ -357,7 +166,7 @@ let ecdsa_verification_ alg public_key r_q s_q msg_len msg =
       false
       end
     else
-      let state = ecdsa_verification_core alg pk hashAsFelem r_q s_q msg_len msg xBuffer in
+      let state = ecdsa_verification_core alg pk z r_q s_q msg_len msg x in
       if state = false then
         begin
         pop_frame ();
@@ -365,7 +174,7 @@ let ecdsa_verification_ alg public_key r_q s_q msg_len msg =
         end
       else
         begin
-        let res = bn_is_eq_vartime4 xBuffer r_q in
+        let res = bn_is_eq_vartime4 x r_q in
         pop_frame ();
         res
         end
